\documentclass{article}
\usepackage{graphicx}
\usepackage{amsmath}
\begin{document}
	\begin{equation}
	Pr\{X = k\} = {n \choose k} p^k (1 - p)^{(n - k)}
	\end{equation}
	\begin{equation}
	E[X] = \sum_{k = 0}^{n} k Pr\{X = k\}
	\end{equation}
	\begin{equation}
	E[X] = \sum_{k = 0}^{n} k {n \choose k} p^k (1 - p)^{(n - k)}
	\end{equation}
	\begin{equation}
	E[X] = \sum_{k = 0}^{n} k \frac{n!}{k!(n - k)!} p^k (1 - p)^{(n - k)}
	\end{equation}
	\begin{equation}
	E[X] = \sum_{k = 0}^{n} \frac{n!}{(k - 1)!(n - k)!} p^k (1 - p)^{(n - k)}
	\end{equation}
	\begin{equation}
	E[X] = np \sum_{k = 0}^{n} \frac{(n - 1)!}{(k - 1)!(n - k)!} p^{(k - 1)} (1 - p)^{(n - k)}
	\end{equation}
	\begin{equation}
	E[X] = np \sum_{k = 0}^{n} \frac{(n - 1)!}{(k - 1)!((n - 1) - (k - 1))!} p^{(k - 1)} (1 - p)^{((n - 1) - (k - 1))}
	\end{equation}
	\begin{equation}
	E[X] = np \sum_{k = 0}^{n} {(n - 1) \choose (k - 1)} p^{(k - 1)} (1 - p)^{((n - 1) - (k - 1))}
	\end{equation}
	\begin{equation}
	E[X] = np \sum_{k = 1}^{n - 1} {(n - 1) \choose (k - 1)} p^{(k - 1)} (1 - p)^{((n - 1) - (k - 1))}
	\end{equation}
	\begin{equation}
	E[X] = np \sum_{a = 0}^{b} {b \choose a} p^{a} (1 - p)^{(b - a)}
	\end{equation}
	\begin{equation}
	E[X] = np \times 1
	\end{equation}
	\begin{equation}
	E[X] = np
	\end{equation}
\end{document}